theories/lang/sharedmem.v
@@ -1,0 +1,149 @@
+From mathcomp Require Import ssreflect ssrfun ssrbool ssrnat seq.
+From mathcomp Require Import eqtype choice finfun finmap tuple.
+From eventstruct Require Import utils inhtype ident relaxed.
+
+Set Implicit Arguments.
+Unset Strict Implicit.
+Unset Printing Implicit Defensive.
+
+Local Open Scope order_scope.
+Local Open Scope fset_scope.
+Local Open Scope ident_scope.
+
+Module SharedMem.
+
+Section Def.
+Context {Addr Val : Type}.
+
+Variant label := 
+  | Read  of Addr & Val 
+  | Write of Addr & Val 
+  | Bot
+  .
+
+Definition typ : label -> Lab.typ :=
+  fun l => match l with
+  | Read  _ _ => Lab.Read
+  | Write _ _ => Lab.Write
+  | Bot       => Lab.Undef
+  end.
+
+(* TODO: define non-option version? *)
+Definition oaddr : label -> option Addr :=
+  fun l => match l with
+  | Read  x _ => Some x
+  | Write x _ => Some x
+  | Bot       => None
+  end.
+
+End Def.
+
+Arguments label _ _ : clear implicits.
+
+Section Encode. 
+Context {Addr Val : Type}.
+
+Definition enc_lab : (label Addr Val) -> Addr * Val + Addr * Val + unit := 
+  fun l => match l with 
+  | Read  x v => inl (inl (x, v))
+  | Write x v => inl (inr (x, v))
+  | Bot       => inr tt
+  end.
+
+Definition dec_lab : Addr * Val + Addr * Val + unit -> (label Addr Val) := 
+  fun l => match l with 
+  | inl (inl (x, v)) => Read x v
+  | inl (inr (x, v)) => Write x v
+  | inr _            => Bot
+  end.
+
+Lemma enc_dec_labK : 
+  cancel enc_lab dec_lab.
+Proof. admit. Admitted.
+
+End Encode.
+
+Module Export Exports.
+
+Definition label_eqMixin (A V : eqType) := 
+  CanEqMixin (@enc_dec_labK A V).
+Canonical label_eqType (A V : eqType) := 
+  Eval hnf in EqType _ (label_eqMixin A V).
+
+Definition label_choiceMixin (A V : choiceType) := 
+  CanChoiceMixin (@enc_dec_labK A V).
+Canonical label_choiceType (A V : choiceType) := 
+  Eval hnf in ChoiceType _ (label_choiceMixin A V).
+
+End Exports.
+
+Module Export LabType.
+Section LabType.
+Context {Addr Val : choiceType}.
+Local Notation label := (label Addr Val).
+Implicit Types (ls : {fset label}) (l : label).
+
+Definition rf : rel label := 
+  fun w r => match w, r with
+  | Write x a, Read y b => (x == y) && (a == b)
+  | _ , _ => false
+  end.
+
+Definition com ws r := 
+  let w := odflt Bot (fset_pick ws) in
+  (#|` ws | == 1) && (rf w r).
+
+Definition cf_typ l1 l2 := 
+  match (typ l1), (typ l2) with 
+  | Lab.Read , Lab.Write  => true
+  | Lab.Write, Lab.Read   => true
+  | Lab.Write, Lab.Write  => true
+  | _        , _          => false
+  end.
+
+Definition cf l1 l2 := 
+  (cf_typ l1 l2) && (oaddr l1 == oaddr l2). 
+
+Definition is_write l := 
+  typ l == Lab.Write.
+
+Definition is_read l := 
+  typ l == Lab.Read.
+
+Lemma is_writeP w :
+  reflect (exists ws r, com ws r /\ w \in ws) (is_write w).
+Proof. 
+  apply/(equivP idP); split; rewrite /com /rf.
+  - move=> isW; exists [fset w].
+    move: w isW; case=> //= x v _.
+    exists (Read x v); rewrite inE; split=> //=.
+    by rewrite fset_pick1 cardfs1 /= !eqxx. 
+  move=> /= [ws] [r] [] /andP[] /cardfs1P[w'] ->.
+  rewrite fset_pick1 inE /=. 
+  by move=> /[swap] /eqP<-; case: w.
+Qed.
+
+Lemma is_readP r :
+  reflect (exists ws, com ws r) (is_read r).
+Proof. 
+  apply/(equivP idP); split; rewrite /com /rf.
+  - case: r=> // x v _.
+    exists [fset (Write x v)].
+    by rewrite fset_pick1 cardfs1 /= !eqxx. 
+  move=> [ws] /andP[] /cardfs1P[w] ->.
+  rewrite fset_pick1 /=. 
+  by case: w; case: r.
+Qed.    
+
+Lemma bot_nwrite : 
+  ~~ is_write Bot.
+Proof. done. Qed.
+
+Lemma bot_nread : 
+  ~~ is_read Bot.
+Proof. done. Qed. 
+
+End LabType.
+End LabType.
+
+End SharedMem.
